1. Fixed up forward_for, the tactic for for-loops (and Sloop) in the   general case; it also takes care (automatically) of several special   cases, not including forward_for_simple_bound.   Test this in progs/verif_min.v and aes/verif_encryption_LL.v
2. Made the forward tactic give much better advice about how to use
 forward_if, forward_while, forward_for, forward_for_simple_bound.
 If you do "forward" on a command that requires one of those, it
 automatically analyzes your situation, and makes specific recommendations
 about what forward-command to use, and how to use it.

3.  Minor changes to the definition of loop1_ret_assert and
  loop2_ret_assert.

4. Fixed up everything in progs, sha, hmac, aes, tweetnacl.

veric/seplog.v
@@ -273,16 +273,16 @@ Qed.
 Definition loop1_ret_assert (Inv: assert) (R: ret_assert) : ret_assert :=
  fun ek vl =>
  match ek with
- | EK_normal => Inv
+ | EK_normal => fun rho => !! (vl = None) && Inv rho
  | EK_break => R EK_normal None
- | EK_continue => Inv
+ | EK_continue => fun rho => !! (vl = None) && Inv rho
  | EK_return => R EK_return vl
  end.
 
 Definition loop2_ret_assert (Inv: assert) (R: ret_assert) : ret_assert :=
  fun ek vl =>
  match ek with
- | EK_normal => Inv
+ | EK_normal => fun rho => !! (vl = None) && Inv rho
  | EK_break => fun _ => FF
  | EK_continue => fun _ => FF
  | EK_return => R EK_return vl
