aes/verif_encryption_LL.v
@@ -55,9 +55,7 @@ Proof.
   match goal with |- context [temp _X2 (Vint ?E)] => change E with (col 2 S0) end.
   match goal with |- context [temp _X3 (Vint ?E)] => change E with (col 3 S0) end.
 
-  forward. unfold Sfor. forward.
-  deadvars!.
-
+  forward. 
   (* ugly hack to avoid type mismatch between
    "(val * (val * list val))%type" and "reptype t_struct_aesctx" *)
   assert (exists (v: reptype t_struct_aesctx), v =
@@ -67,12 +65,13 @@ Proof.
   as EE by (eexists; reflexivity).
 
   destruct EE as [vv EE].
-
   remember (mbed_tls_enc_rounds 12 S0 buf 4) as S12.
-  apply semax_pre with (P' := 
-  (EX i: Z, PROP ( 
+
+  forward_for 
+  (* Loop Invariant *)  
+  (fun i:Z => PROP ( 
      0 <= i <= 6
-  ) LOCAL (
+   ) LOCAL (
      temp _i (Vint (Int.repr i));
      temp _RK (field_address t_struct_aesctx [ArraySubsc (52 - i*8); StructField _buf] ctx);
      temp _X3 (Vint (col 3 (mbed_tls_enc_rounds (12 - 2 * (Z.to_nat i)) S0 buf 4)));
@@ -86,27 +85,9 @@ Proof.
      tables_initialized tables;
      data_at in_sh (tarray tuchar 16) (map Vint (map Int.repr plaintext)) input;
      data_at ctx_sh t_struct_aesctx vv ctx
-  ))).
-  { subst vv. Exists 6. entailer!. }
-
-  eapply semax_seq' with (P' :=
-  PROP ( )
-  LOCAL (
-     temp _RK (field_address t_struct_aesctx [ArraySubsc 52; StructField _buf] ctx);
-     temp _X3 (Vint (col 3 S12));
-     temp _X2 (Vint (col 2 S12));
-     temp _X1 (Vint (col 1 S12));
-     temp _X0 (Vint (col 0 S12));
-     temp _output output;
-     gvar _tables tables
-  ) SEP (
-     data_at_ out_sh (tarray tuchar 16) output;
-     tables_initialized tables;
-     data_at in_sh (tarray tuchar 16) (map Vint (map Int.repr plaintext)) input;
-     data_at ctx_sh t_struct_aesctx vv ctx 
-  )).
-  { apply semax_loop with (
-  (EX i: Z, PROP ( 
+  ))
+  (* PreInc invariant *)
+   (fun i: Z => PROP ( 
      0 < i <= 6
   ) LOCAL (
      temp _i (Vint (Int.repr i));
@@ -122,54 +103,54 @@ Proof.
      tables_initialized tables;
      data_at in_sh (tarray tuchar 16) (map Vint (map Int.repr plaintext)) input;
      data_at ctx_sh t_struct_aesctx vv ctx
-  ))).
-  { (* loop body *) 
-  Intro i.
-  reassoc_seq.
-  forward_if
-  (EX i: Z, PROP ( 
-     0 < i <= 6
-  ) LOCAL (
-     temp _i (Vint (Int.repr i));
-     temp _RK (field_address t_struct_aesctx [ArraySubsc (52 - i*8); StructField _buf] ctx);
-     temp _X3 (Vint (col 3 (mbed_tls_enc_rounds (12 - 2 * (Z.to_nat i)) S0 buf 4)));
-     temp _X2 (Vint (col 2 (mbed_tls_enc_rounds (12 - 2 * (Z.to_nat i)) S0 buf 4)));
-     temp _X1 (Vint (col 1 (mbed_tls_enc_rounds (12 - 2 * (Z.to_nat i)) S0 buf 4)));
-     temp _X0 (Vint (col 0 (mbed_tls_enc_rounds (12 - 2 * (Z.to_nat i)) S0 buf 4)));
+  ))
+  (* Loop postcondition *)
+  (PROP() LOCAL (
+     temp _RK (field_address t_struct_aesctx [ArraySubsc 52; StructField _buf] ctx);
+     temp _X3 (Vint (col 3 S12));
+     temp _X2 (Vint (col 2 S12));
+     temp _X1 (Vint (col 1 S12));
+     temp _X0 (Vint (col 0 S12));
      temp _output output;
      gvar _tables tables
   ) SEP (
      data_at_ out_sh (tarray tuchar 16) output;
      tables_initialized tables;
      data_at in_sh (tarray tuchar 16) (map Vint (map Int.repr plaintext)) input;
-     data_at ctx_sh t_struct_aesctx vv ctx
+     data_at ctx_sh t_struct_aesctx vv ctx 
   )).
-  { (* then-branch: Sskip to body *)
-  Intros. forward. Exists i.
-(*  rewrite Int.signed_repr in *; [ | repable_signed ]. (* TODO floyd why is this not automatic? *) *)
-  entailer!.
-  }
-  { (* else-branch: exit loop *)
-  Intros.
-(*  rewrite Int.signed_repr in *; [ | repable_signed ]. (* TODO floyd why is this not automatic? *) *)
-  forward. assert (i = 0) by omega. subst i.
-  change (52 - 0 * 8) with 52.
-  change (12 - 2 * Z.to_nat 0)%nat with 12%nat.
-  replace (mbed_tls_enc_rounds 12 S0 buf 4) with S12 by reflexivity. (* interestingly, if we use
-     "change" instead of "replace", it takes much longer *)
-  entailer!.
-  }
-  { (* rest: loop body *)
-  clear i. Intro i. Intros. 
+* (* initializer establishes loop invariant *)
+ forward. Exists 6. entailer!.
+* (* loop-test typechecks *)
+ entailer!.
+* (*  loop body *)
+  rename a into i.
+  assert (0 < i <= 6) by (clear - H1 H2; omega).
   unfold tables_initialized. subst vv.
+  reassoc_seq.
   subst MORE_COMMANDS POSTCONDITION. unfold abbreviate.
   change Delta with (encryption_loop_body_Delta Delta_specs).
+  fold encryption_loop_body.
+  eapply semax_post_flipped.
   simple eapply encryption_loop_body_proof; eauto.
-  }} { (* loop decr *)
-  Intro i. forward. unfold loop2_ret_assert. Exists (i-1). entailer!.
-  }} 
-
-(** AFTER THE LOOP **)
+  (* the next few lines should not be necessary if the statement
+    of encryption_loop_body_proof is adjusted. *)
+  clear.
+  intros. match goal with |- 
+     context [loop1_ret_assert ?PP (normal_ret_assert ?QQ)] =>
+     set (P:=PP); set (Q := QQ)
+   end.
+  apply andp_left2.
+  unfold loop1_ret_assert, normal_ret_assert, overridePost; destruct ek; auto.
+  rewrite if_true by auto. rewrite !prop_true_andp by auto.
+  subst Q.  solve [auto].
+  apply derives_extract_prop; intro Hx; inv Hx.
+* (* loop decr *)
+  rename a into i. forward. Exists (i-1). entailer!.
+* (* after the loop, entailment *)
+ assert (a=0) by omega. clear H1 H2; subst a.
+ entailer!.
+* (** AFTER THE LOOP **)
 subst vv.
 abbreviate_semax.
 subst MORE_COMMANDS POSTCONDITION; unfold abbreviate.
